Verbatim/memo/memo.v
@@ -1,0 +1,29 @@
+Require Import List.
+Import ListNotations.
+
+From Verbatim Require Import state.
+
+Module Type MEMO (Import STT : state.T).
+
+  Import STT.
+  Import STT.Ty.
+
+  Parameter Memo : Type.
+  Parameter emptyMemo : Memo.
+  Parameter set_Memo : Memo -> State -> String -> option(String * String) -> Memo.
+  Parameter get_Memo : Memo -> State -> String -> option (option (String * String)).
+
+  Parameter correct_Memo : forall M stt z o, get_Memo (set_Memo M stt z o) stt z = Some (o).
+  Parameter correct_emptyMemo : forall stt z, get_Memo emptyMemo stt z = None.
+
+End MEMO.
+
+(*Module MemoDefsFn (STT : state.T) (MEM : MEMO STT).*)
+
+Module Type T.
+  Declare Module STT : state.T.
+  Declare Module Ty : MEMO STT.
+  Export STT.
+  Export STT.Ty.
+  Export Ty.
+End T.
