Verbatim/memo/memocore.v
@@ -1,0 +1,15 @@
+Require Import List.
+Import ListNotations.
+Require Import PeanoNat.
+Require Import Coq.omega.Omega.
+
+From VLG Require Import ltac.
+From VLG Require Import coredefs.
+
+Parameter Memo : Type.
+Parameter emptyMemo : Memo.
+Parameter set_Memo : Memo -> State -> String -> option(Prefix * Suffix) -> Memo.
+Parameter get_Memo : Memo -> State -> String -> option (option (Prefix * Suffix)).
+
+Hypothesis correct_Memo : forall M stt z o, get_Memo (set_Memo M stt z o) stt z = Some (o).
+Hypothesis correct_emptyMemo : forall stt z, get_Memo emptyMemo stt z = None.
