Verbatim/memo/memolexer.v
@@ -1,0 +1,269 @@
+Require Import List.
+Import ListNotations.
+Require Import PeanoNat.
+Require Import Coq.omega.Omega.
+
+From VLG Require Import ltac.
+From VLG Require Import coredefs.
+From VLG Require Import spec.
+From VLG Require Import prefixer.
+From VLG Require Import lexer.
+From VLG Require Import lemmas.
+From VLG Require Import memocore.
+From VLG Require Import memopref.
+From VLG Require Import memospec.
+
+(* Lexer *)
+
+
+Lemma memo_len_const : forall n Ms rules code Ms' l0,
+    n = length Ms'
+    -> length Ms = length rules
+    -> max_prefs__M Ms code rules = (Ms', l0)
+    -> length Ms' = length Ms.
+Proof.
+  induction n; intros; destruct rules; destruct Ms; destruct Ms'; destruct l0;
+      try(simpl in *; auto; discriminate);
+      try(unfold max_prefs__M in *; simpl in *; repeat dm; repeat inj_all; subst; discriminate).
+  + simpl in *. injection H; intros; clear H. injection H0; intros; clear H0.
+    apply cons_mprefs__M in H1. destruct H1. eapply IHn in H2; eauto.
+Qed.
+
+Lemma labeled_len_const : forall n Ms rules code Ms' l0,
+    n = length Ms'
+    -> length Ms = length rules
+    -> max_prefs__M Ms code rules = (Ms', l0)
+    -> length Ms' = length l0.
+Proof.
+  induction n; intros; destruct rules; destruct Ms; destruct Ms'; destruct l0;
+      try(simpl in *; auto; discriminate);
+      try(unfold max_prefs__M in *; simpl in *; repeat dm; repeat inj_all; subst; discriminate).
+  + simpl in *. injection H; intros; clear H. injection H0; intros; clear H0.
+    apply cons_mprefs__M in H1. destruct H1. eapply IHn in H2; eauto.
+Qed.
+
+Lemma all_lens_const' : forall n Ms rules code Ms' l0,
+    n = length Ms'
+    -> length Ms = length rules
+    -> max_prefs__M Ms code rules = (Ms', l0)
+    -> length Ms' = length Ms /\ length Ms' = length l0.
+Proof.
+  intros. split.
+  - eapply memo_len_const; eauto.
+  - eapply labeled_len_const; eauto.
+Qed.
+
+Lemma all_lens_const : forall Ms rules code Ms' l0,
+    length Ms = length rules
+    -> max_prefs__M Ms code rules = (Ms', l0)
+    -> length Ms' = length Ms /\ length Ms' = length l0.
+Proof.
+  intros. eapply all_lens_const'; eauto.
+Qed.
+
+Lemma mprefs__M_associates :
+  forall n rules Ms Ms' code (l0 : list (Label * option (Prefix * Suffix))) M M' o label ru,
+  length Ms = length rules
+  -> max_prefs__M Ms code rules = (Ms', l0)
+  -> n < length Ms'
+  -> nth n Ms emptyMemo = M
+  -> nth n Ms' emptyMemo = M'
+  -> nth n l0 ([], None) = (label, o)
+  -> nth n rules ([], defState) = (label, ru)
+  -> max_pref_fn__M M code ru = (M', o).
+Proof.
+  induction n; intros; destruct Ms; destruct Ms'; destruct l0; destruct rules;
+      try(simpl in *; omega);
+      try(rewrite nil_mprefs__M in *; repeat inj_all; discriminate);
+      try(simpl in *; repeat inj_all; unfold max_prefs__M in *; simpl in *;
+          repeat dm; repeat inj_all; discriminate).
+    + simpl in *. subst. unfold max_prefs__M in *. simpl in *.
+      repeat dm. repeat inj_all. auto.
+    + simpl in *. injection H; intros; clear H.
+      apply lt_S_n in H1. eapply IHn; eauto. eapply cons_mprefs__M; eauto.
+Qed.
+
+
+Lemma nth_labels_match'' : forall m n rules Ms code Ms' l0 o ru label label',
+    m = length rules
+    -> length Ms = length rules
+    -> length rules = length l0
+    -> length Ms' = length Ms
+    -> n < length Ms'
+    -> max_prefs__M Ms code rules = (Ms', l0)
+    -> nth n l0 ([], None) = (label, o)
+    -> nth n rules ([], defState) = (label', ru)
+    -> label = label'.
+Proof.
+  induction m; intros; destruct Ms; destruct rules; destruct Ms'; destruct l0; destruct n;
+    try(simpl in *; omega).
+  - apply cons_mprefs__M in H4. destruct H4. clear H7. simpl in *.
+    unfold max_prefs__M in H4. simpl in *. repeat dm; repeat inj_all. auto.
+  - simpl in *.
+    apply Nat.succ_inj in H.  apply Nat.succ_inj in H0.
+    apply Nat.succ_inj in H1. apply Nat.succ_inj in H2.
+    apply lt_S_n in H3.
+    apply cons_mprefs__M in H4. destruct H4.
+    eapply IHm; eauto.
+Qed.
+
+Lemma nth_labels_match' : forall m n rules Ms code Ms' l0 o ru label label',
+    m = length rules
+    -> length Ms = length rules
+    -> n < length Ms'
+    -> max_prefs__M Ms code rules = (Ms', l0)
+    -> nth n l0 ([], None) = (label, o)
+    -> nth n rules ([], defState) = (label', ru)
+    -> label = label'.
+Proof.
+  intros.
+  assert(L := all_lens_const Ms rules code Ms' l0 H0 H2). destruct L.
+  eapply nth_labels_match''; eauto. omega.
+Qed.
+
+Lemma nth_labels_match : forall n rules Ms code Ms' l0 o ru label label',
+    max_prefs__M Ms code rules = (Ms', l0)
+    -> length Ms = length rules
+    -> n < length Ms'
+    -> nth n l0 ([], None) = (label, o)
+    -> nth n rules ([], defState) = (label', ru)
+    -> label = label'.
+Proof.
+  intros. eapply nth_labels_match'; eauto.
+Qed.
+
+Lemma lexy_closure : 
+  forall code rules M o M',
+  lexy M
+  -> max_pref_fn__M M code rules = (M', o)
+  -> lexy M'.
+Proof.
+  induction code; intros.
+  - simpl in H0. repeat dm; repeat inj_all; auto; discriminate.
+  - simpl in H0. repeat dm; repeat inj_all; auto;
+                   try(eapply IHcode; eauto).
+Qed.
+
+Lemma lexy_list_closure : 
+  forall code rules Ms l0 Ms',
+  lexy_list Ms
+  -> length Ms = length rules
+  -> max_prefs__M Ms code rules = (Ms', l0)
+  -> lexy_list Ms'.
+Proof.
+  intros. unfold lexy_list in *. intros M' H2.
+  apply In_nth with (d := emptyMemo) in H2. destruct H2 as [n]. destruct H2.
+  assert(L := all_lens_const Ms rules code Ms' l0 H0 H1). destruct L.
+  assert(exists M, nth n Ms emptyMemo = M).
+  { eexists; eauto. }
+  destruct H6 as [M].
+  assert(exists label o, nth n l0 ([], None) = (label, o)).
+  { destruct (nth n l0 ([], None)). eexists; eauto. }
+  destruct H7 as [label]. destruct H7 as [o].
+  assert(exists label' ru, nth n rules ([], defState) = (label', ru)).
+  { destruct (nth n rules ([], defState)). eexists; eauto. }
+  destruct H8 as [label']. destruct H8 as [ru].
+  assert(label = label').
+  { eapply nth_labels_match; eauto. }
+  rewrite H9 in *. clear H9.
+  eapply mprefs__M_associates in H0; eauto.
+
+  assert(Hlen : length Ms = length Ms').
+  { omega. }
+  
+  rewrite <- Hlen in H2.
+  apply nth_In with (d:=emptyMemo) in H2. rewrite H6 in H2. apply H in H2.
+  eapply lexy_closure; eauto.
+Qed.
+
+Lemma len_recursive_call :
+  forall code rules label s l suffix Ms Ms',
+    length Ms = length rules
+    -> max_of_prefs__M (max_prefs__M Ms code rules) = (Ms', label, Some (s :: l, suffix))
+    -> length Ms' = length rules.
+Proof.
+  intros. destruct (max_prefs__M Ms code rules) eqn:E.
+  assert(l0 = Ms').
+  {
+    simpl in H0. repeat dm. injection H0; auto.
+  }
+  subst. clear H0.
+  assert(L := all_lens_const Ms rules code Ms' l1 H E). destruct L. omega.
+Qed.
+  
+
+Lemma lexy_recursive_call_gen :
+  forall code rules Ms label o Ms',
+  lexy_list Ms
+  -> length Ms = length rules
+  -> max_of_prefs__M (max_prefs__M Ms code rules) = (Ms', label, o)
+  -> lexy_list Ms'.
+Proof.
+  intros. destruct (max_prefs__M Ms code rules) eqn:E.
+  assert(l = Ms').
+  {
+    simpl in H1. repeat dm. injection H1; auto.
+  }
+  subst. clear H1.
+  eapply lexy_list_closure in H; eauto.
+Qed.
+
+
+Lemma lexy_recursive_call :
+  forall code rules Ms label s l suffix Ms',
+  lexy_list Ms
+  -> length Ms = length rules
+  -> max_of_prefs__M (max_prefs__M Ms code rules) = (Ms', label, Some (s :: l, suffix))
+  -> lexy_list Ms'.
+Proof.
+  intros. eapply lexy_recursive_call_gen in H; eauto.
+Qed.
+  
+Lemma acc_helper__M : forall Ms code rules Ms' label o,
+    lexy_list Ms
+    -> length Ms = length rules
+    -> max_of_prefs__M (max_prefs__M Ms code rules) = (Ms', label, o)
+    -> max_of_prefs (max_prefs code rules) = (label, o).
+Proof.
+  intros. destruct (max_prefs code rules) eqn:E; destruct (max_prefs__M Ms code rules) eqn:E1.
+  - simpl in *. repeat dm; repeat inj_all; subst. eapply mprefs_memo_F in H; eauto.
+    + rewrite E in H. subst. simpl in E0. auto.
+  - simpl in *. repeat dm; repeat inj_all; subst. eapply mprefs_memo_F in H; eauto.
+    rewrite E in H. subst. simpl in E0. auto.
+Qed.
+
+Lemma acc_recursive_call__M :
+  forall code rules label s l suffix Ms Ms',
+    Acc lt (length code)
+    -> lexy_list Ms
+    -> length Ms = length rules
+    -> max_of_prefs__M (max_prefs__M Ms code rules) = (Ms', label, Some (s :: l, suffix))
+    -> Acc lt (length suffix).
+Proof.
+  intros. eapply acc_helper__M in H0; eauto; eapply acc_recursive_call; eauto.
+Defined.
+
+Fixpoint lex'__M
+         (Ms : list Memo)
+         (rules : list (sRule))
+         (code : String)
+         (Ha : Acc lt (length code))
+         (Hlexy : lexy_list Ms)
+         (Hlen : length Ms = length rules)
+         {struct Ha} : (list Memo) * (list Token) * String :=
+  match max_of_prefs__M (max_prefs__M Ms code rules) as mpref'
+        return max_of_prefs__M (max_prefs__M Ms code rules) = mpref' -> _
+  with
+  | (Ms', _, None) => fun _ => (Ms', [], code) (* Code cannot be processed further *)
+  | (Ms', _, Some ([], _)) => fun _ => (Ms', [], code) (* Code cannot be processed further *)
+  | (Ms', label, Some (ph :: pt, suffix)) =>
+    fun Heq =>
+      match (lex'__M Ms' rules suffix
+                   (acc_recursive_call__M _ _ _ _ _ _ _ _ Ha Hlexy Hlen Heq)
+                   (lexy_recursive_call _ _ _ _ _ _ _ _ Hlexy Hlen Heq)
+                   (len_recursive_call _ _ _ _ _ _ _ _ Hlen Heq)
+            )
+      with
+      | (Ms'', lexemes, rest) => (Ms'', ((label, ph :: pt) :: lexemes), rest)
+      end
+  end eq_refl.
